meta/HelperTactics.fst
@@ -1,0 +1,81 @@
+module HelperTactics
+
+include FStar.Tactics.V2
+include FStar.Reflection.Typing
+
+let must (x : ret_t 'a) : Tac 'a =
+  match x with
+  | Some v, _ -> v
+  | None, [] ->
+    fail ("must failed, no issues?")
+  | None, i::_ ->
+    fail ("must failed: " ^ FStar.Issue.render_issue i)
+
+(* Metaprograms with partial correctness *)
+effect TacP (a:Type) (pre:prop) (post : a -> prop) =
+  TacH a (requires (fun _ -> pre))
+         (ensures (fun _ps r ->
+           match r with
+           | FStar.Stubs.Tactics.Result.Success v ps -> post v
+           | _ -> True))
+
+(** ** Help with quotations **)
+let qunit : term = `()
+
+(** ** Static Typing **)
+let valid (g:env) (phi:term) : prop =
+  squash (tot_typing g qunit (mk_squash phi))
+
+let valid_wtf (g:env) (phi:term) 
+  : Lemma (requires valid g phi)
+          (ensures squash (tot_typing g qunit (mk_squash phi)))
+  = let goal = squash (tot_typing g qunit (mk_squash phi)) in
+    assert (valid g phi ==> goal) by (compute ()); /// WHY????
+    () // ????
+
+let same_typing (t0 t1 : term) : prop =
+  forall g c typ. typing g t0 (c, typ) ==> typing g t1 (c, typ)
+
+let same_valid (t0 t1 : term) : prop =
+  forall g. valid g t0 ==> valid g t1
+
+let mk_eq2 (ty t1 t2 : term) : Tot term =
+  mk_app (`Prims.eq2) [(ty, Q_Implicit); (t1, Q_Explicit); (t2, Q_Explicit)]	
+
+(** ** Normalize **)
+val typed_norm_term_env :
+  ty:typ ->
+  g:env ->
+  list norm_step ->
+  t0:term{tot_typing g t0 ty} ->
+  Tac (t1:term{same_typing t0 t1 /\ valid g (mk_eq2 ty t0 t1)})
+let typed_norm_term_env ty g steps t0 =
+  let t1 = norm_term_env g steps t0 in
+  admit(); // can't prove this, we should strengthen norm_term_env in F* library
+  t1
+
+(** ** Dynamic Typing **)
+let dyn_typing (#g #ty #t : _) () : Tac (tot_typing g t ty) =
+  let tok = must <| core_check_term g t ty E_Total in
+  T_Token _ _ _ (Squash.return_squash tok)
+
+let type_dynamically g ty t : TacP unit (requires True) (ensures fun _ -> squash (tot_typing g ty t)) =
+  let ht : tot_typing g ty t = dyn_typing () in
+  Squash.return_squash ht
+
+let assert_dynamically g phi : TacP unit (requires True) (ensures fun _ -> squash (valid g phi)) =
+  let ht : tot_typing g qunit (mk_squash phi) = dyn_typing () in
+  Squash.return_squash ht
+
+
+
+let rec fold_left (f:'a -> 'b -> 'a) (acc:'a) (l:list 'b) : Tot 'a (decreases l)=
+  match l with
+  | [] -> acc
+  | hd::tl -> fold_left f (f acc hd) tl
+
+let fv_to_string (fv:fv) : string =
+  match inspect_fv fv with
+  | [] -> ""
+  | h::[] -> h
+  | h::tl -> fold_left (fun x y -> x ^ "." ^ y) h tl
